Mica/Stdlib/FloatStd.lean
@@ -115,6 +115,8 @@ def floatAbsB : Pure.Unary where
   arg      := .float
   res      := .float
   f        := FloatBits.abs
+  dom      := fun _ => True
+  pre      := none
   defAxiom := floatAbsDefAxiom
 
 def floatAbs : Intrinsic := floatAbsB.toIntrinsic
@@ -123,12 +125,14 @@ def floatAbs : Intrinsic := floatAbsB.toIntrinsic
 @[simp] theorem floatAbs_arity : floatAbs.arity = .one := rfl
 
 def floatAbsLawful : floatAbsB.Lawful where
-  argL       := Embedding.lawfulFloat
-  resL       := Embedding.lawfulFloat
-  specBaseWf := by apply PredTrans.checkWf_ok; rfl
-  defWf      := by apply Formula.checkWf_ok; rfl
-  typeWf     := by apply Formula.checkWf_ok; rfl
-  defEval    := by intrinsic_def_eval [unTerm, floatAbsB, floatAbsDefAxiom]; intros; rfl
+  argL         := Embedding.lawfulFloat
+  resL         := Embedding.lawfulFloat
+  domSound     := fun _ _ _ => True.intro
+  semWellTyped := fun _ _ _ _ => .rfl
+  specBaseWf   := by apply PredTrans.checkWf_ok; rfl
+  defWf        := by apply Formula.checkWf_ok; rfl
+  typeWf       := by intro φ h; injection h with h; subst h; apply Formula.checkWf_ok; rfl
+  defEval      := by intrinsic_def_eval [unTerm, floatAbsB, floatAbsDefAxiom]; intros; rfl
 
 instance : IntrinsicSound [floatAbs] floatAbs := floatAbsLawful.sound
 
@@ -143,6 +147,8 @@ def floatNegB : Pure.Unary where
   arg      := .float
   res      := .float
   f        := FloatBits.neg
+  dom      := fun _ => True
+  pre      := none
   defAxiom := floatNegDefAxiom
 
 def floatNeg : Intrinsic := floatNegB.toIntrinsic
@@ -151,12 +157,14 @@ def floatNeg : Intrinsic := floatNegB.toIntrinsic
 @[simp] theorem floatNeg_arity : floatNeg.arity = .one := rfl
 
 def floatNegLawful : floatNegB.Lawful where
-  argL       := Embedding.lawfulFloat
-  resL       := Embedding.lawfulFloat
-  specBaseWf := by apply PredTrans.checkWf_ok; rfl
-  defWf      := by apply Formula.checkWf_ok; rfl
-  typeWf     := by apply Formula.checkWf_ok; rfl
-  defEval    := by intrinsic_def_eval [unTerm, floatNegB, floatNegDefAxiom]; intros; rfl
+  argL         := Embedding.lawfulFloat
+  resL         := Embedding.lawfulFloat
+  domSound     := fun _ _ _ => True.intro
+  semWellTyped := fun _ _ _ _ => .rfl
+  specBaseWf   := by apply PredTrans.checkWf_ok; rfl
+  defWf        := by apply Formula.checkWf_ok; rfl
+  typeWf       := by intro φ h; injection h with h; subst h; apply Formula.checkWf_ok; rfl
+  defEval      := by intrinsic_def_eval [unTerm, floatNegB, floatNegDefAxiom]; intros; rfl
 
 instance : IntrinsicSound [floatNeg] floatNeg := floatNegLawful.sound
 
@@ -171,6 +179,8 @@ def floatSqrtB : Pure.Unary where
   arg      := .float
   res      := .float
   f        := FloatBits.sqrt
+  dom      := fun _ => True
+  pre      := none
   defAxiom := floatSqrtDefAxiom
 
 def floatSqrt : Intrinsic := floatSqrtB.toIntrinsic
@@ -179,12 +189,14 @@ def floatSqrt : Intrinsic := floatSqrtB.toIntrinsic
 @[simp] theorem floatSqrt_arity : floatSqrt.arity = .one := rfl
 
 def floatSqrtLawful : floatSqrtB.Lawful where
-  argL       := Embedding.lawfulFloat
-  resL       := Embedding.lawfulFloat
-  specBaseWf := by apply PredTrans.checkWf_ok; rfl
-  defWf      := by apply Formula.checkWf_ok; rfl
-  typeWf     := by apply Formula.checkWf_ok; rfl
-  defEval    := by intrinsic_def_eval [unTerm, floatSqrtB, floatSqrtDefAxiom]; intros; rfl
+  argL         := Embedding.lawfulFloat
+  resL         := Embedding.lawfulFloat
+  domSound     := fun _ _ _ => True.intro
+  semWellTyped := fun _ _ _ _ => .rfl
+  specBaseWf   := by apply PredTrans.checkWf_ok; rfl
+  defWf        := by apply Formula.checkWf_ok; rfl
+  typeWf       := by intro φ h; injection h with h; subst h; apply Formula.checkWf_ok; rfl
+  defEval      := by intrinsic_def_eval [unTerm, floatSqrtB, floatSqrtDefAxiom]; intros; rfl
 
 instance : IntrinsicSound [floatSqrt] floatSqrt := floatSqrtLawful.sound
 
@@ -199,6 +211,8 @@ def floatIsNanB : Pure.Unary where
   arg      := .float
   res      := .bool
   f        := FloatBits.isNaN
+  dom      := fun _ => True
+  pre      := none
   defAxiom := floatIsNanDefAxiom
 
 def floatIsNan : Intrinsic := floatIsNanB.toIntrinsic
@@ -207,12 +221,14 @@ def floatIsNan : Intrinsic := floatIsNanB.toIntrinsic
 @[simp] theorem floatIsNan_arity : floatIsNan.arity = .one := rfl
 
 def floatIsNanLawful : floatIsNanB.Lawful where
-  argL       := Embedding.lawfulFloat
-  resL       := Embedding.lawfulBool
-  specBaseWf := by apply PredTrans.checkWf_ok; rfl
-  defWf      := by apply Formula.checkWf_ok; rfl
-  typeWf     := by apply Formula.checkWf_ok; rfl
-  defEval    := by intrinsic_def_eval [unTerm, floatIsNanB, floatIsNanDefAxiom]; intros; rfl
+  argL         := Embedding.lawfulFloat
+  resL         := Embedding.lawfulBool
+  domSound     := fun _ _ _ => True.intro
+  semWellTyped := fun _ _ _ _ => .rfl
+  specBaseWf   := by apply PredTrans.checkWf_ok; rfl
+  defWf        := by apply Formula.checkWf_ok; rfl
+  typeWf       := by intro φ h; injection h with h; subst h; apply Formula.checkWf_ok; rfl
+  defEval      := by intrinsic_def_eval [unTerm, floatIsNanB, floatIsNanDefAxiom]; intros; rfl
 
 instance : IntrinsicSound [floatIsNan] floatIsNan := floatIsNanLawful.sound
 
@@ -231,6 +247,8 @@ def floatIsFiniteB : Pure.Unary where
   arg      := .float
   res      := .bool
   f        := FloatBits.isFinite
+  dom      := fun _ => True
+  pre      := none
   defAxiom := floatIsFiniteDefAxiom
 
 def floatIsFinite : Intrinsic := floatIsFiniteB.toIntrinsic
@@ -239,12 +257,14 @@ def floatIsFinite : Intrinsic := floatIsFiniteB.toIntrinsic
 @[simp] theorem floatIsFinite_arity : floatIsFinite.arity = .one := rfl
 
 def floatIsFiniteLawful : floatIsFiniteB.Lawful where
-  argL       := Embedding.lawfulFloat
-  resL       := Embedding.lawfulBool
-  specBaseWf := by apply PredTrans.checkWf_ok; rfl
-  defWf      := by apply Formula.checkWf_ok; rfl
-  typeWf     := by apply Formula.checkWf_ok; rfl
-  defEval    := by intrinsic_def_eval [unTerm, floatIsFiniteB, floatIsFiniteDefAxiom, FloatBits.isFinite]; intros; rfl
+  argL         := Embedding.lawfulFloat
+  resL         := Embedding.lawfulBool
+  domSound     := fun _ _ _ => True.intro
+  semWellTyped := fun _ _ _ _ => .rfl
+  specBaseWf   := by apply PredTrans.checkWf_ok; rfl
+  defWf        := by apply Formula.checkWf_ok; rfl
+  typeWf       := by intro φ h; injection h with h; subst h; apply Formula.checkWf_ok; rfl
+  defEval      := by intrinsic_def_eval [unTerm, floatIsFiniteB, floatIsFiniteDefAxiom, FloatBits.isFinite]; intros; rfl
 
 instance : IntrinsicSound [floatIsFinite] floatIsFinite := floatIsFiniteLawful.sound
 
@@ -259,6 +279,8 @@ def floatOfIntB : Pure.Unary where
   arg      := .int
   res      := .float
   f        := FloatBits.ofInt
+  dom      := fun _ => True
+  pre      := none
   defAxiom := floatOfIntDefAxiom
 
 def floatOfInt : Intrinsic := floatOfIntB.toIntrinsic
@@ -267,12 +289,14 @@ def floatOfInt : Intrinsic := floatOfIntB.toIntrinsic
 @[simp] theorem floatOfInt_arity : floatOfInt.arity = .one := rfl
 
 def floatOfIntLawful : floatOfIntB.Lawful where
-  argL       := Embedding.lawfulInt
-  resL       := Embedding.lawfulFloat
-  specBaseWf := by apply PredTrans.checkWf_ok; rfl
-  defWf      := by apply Formula.checkWf_ok; rfl
-  typeWf     := by apply Formula.checkWf_ok; rfl
-  defEval    := by intrinsic_def_eval [unTerm, floatOfIntB, floatOfIntDefAxiom]; intros; rfl
+  argL         := Embedding.lawfulInt
+  resL         := Embedding.lawfulFloat
+  domSound     := fun _ _ _ => True.intro
+  semWellTyped := fun _ _ _ _ => .rfl
+  specBaseWf   := by apply PredTrans.checkWf_ok; rfl
+  defWf        := by apply Formula.checkWf_ok; rfl
+  typeWf       := by intro φ h; injection h with h; subst h; apply Formula.checkWf_ok; rfl
+  defEval      := by intrinsic_def_eval [unTerm, floatOfIntB, floatOfIntDefAxiom]; intros; rfl
 
 instance : IntrinsicSound [floatOfInt] floatOfInt := floatOfIntLawful.sound
 
@@ -285,9 +309,12 @@ private def binFloatDefAxiom (sym : FOL.Symbol .two) (op : BinOp .float .float .
 def floatAddB : Pure.Binary where
   name     := "float_add"
   path     := some ("Float", ["add"])
-  arg      := .float
+  arg₁     := .float
+  arg₂     := .float
   res      := .float
   f        := FloatBits.add
+  dom      := fun _ _ => True
+  pre      := none
   defAxiom := binFloatDefAxiom floatAddSym .fpAdd
 
 def floatAdd : Intrinsic := floatAddB.toIntrinsic
@@ -296,21 +323,27 @@ def floatAdd : Intrinsic := floatAddB.toIntrinsic
 @[simp] theorem floatAdd_arity : floatAdd.arity = .two := rfl
 
 def floatAddLawful : floatAddB.Lawful where
-  argL       := Embedding.lawfulFloat
-  resL       := Embedding.lawfulFloat
-  specBaseWf := by apply PredTrans.checkWf_ok; rfl
-  defWf      := by apply Formula.checkWf_ok; rfl
-  typeWf     := by apply Formula.checkWf_ok; rfl
-  defEval    := by intrinsic_def_eval [binTerm, floatAddB, floatAddSym, binFloatDefAxiom]; intros; rfl
+  argL₁        := Embedding.lawfulFloat
+  argL₂        := Embedding.lawfulFloat
+  resL         := Embedding.lawfulFloat
+  domSound     := fun _ _ _ _ => True.intro
+  semWellTyped := fun _ _ _ _ _ => sep_emp.1
+  specBaseWf   := by apply PredTrans.checkWf_ok; rfl
+  defWf        := by apply Formula.checkWf_ok; rfl
+  typeWf       := by intro φ h; injection h with h; subst h; apply Formula.checkWf_ok; rfl
+  defEval      := by intrinsic_def_eval [binTerm, floatAddB, floatAddSym, binFloatDefAxiom]; intros; rfl
 
 instance : IntrinsicSound [floatAdd] floatAdd := floatAddLawful.sound
 
 def floatSubB : Pure.Binary where
   name     := "float_sub"
   path     := some ("Float", ["sub"])
-  arg      := .float
+  arg₁     := .float
+  arg₂     := .float
   res      := .float
   f        := FloatBits.sub
+  dom      := fun _ _ => True
+  pre      := none
   defAxiom := binFloatDefAxiom floatSubSym .fpSub
 
 def floatSub : Intrinsic := floatSubB.toIntrinsic
@@ -319,21 +352,27 @@ def floatSub : Intrinsic := floatSubB.toIntrinsic
 @[simp] theorem floatSub_arity : floatSub.arity = .two := rfl
 
 def floatSubLawful : floatSubB.Lawful where
-  argL       := Embedding.lawfulFloat
-  resL       := Embedding.lawfulFloat
-  specBaseWf := by apply PredTrans.checkWf_ok; rfl
-  defWf      := by apply Formula.checkWf_ok; rfl
-  typeWf     := by apply Formula.checkWf_ok; rfl
-  defEval    := by intrinsic_def_eval [binTerm, floatSubB, floatSubSym, binFloatDefAxiom]; intros; rfl
+  argL₁        := Embedding.lawfulFloat
+  argL₂        := Embedding.lawfulFloat
+  resL         := Embedding.lawfulFloat
+  domSound     := fun _ _ _ _ => True.intro
+  semWellTyped := fun _ _ _ _ _ => sep_emp.1
+  specBaseWf   := by apply PredTrans.checkWf_ok; rfl
+  defWf        := by apply Formula.checkWf_ok; rfl
+  typeWf       := by intro φ h; injection h with h; subst h; apply Formula.checkWf_ok; rfl
+  defEval      := by intrinsic_def_eval [binTerm, floatSubB, floatSubSym, binFloatDefAxiom]; intros; rfl
 
 instance : IntrinsicSound [floatSub] floatSub := floatSubLawful.sound
 
 def floatMulB : Pure.Binary where
   name     := "float_mul"
   path     := some ("Float", ["mul"])
-  arg      := .float
+  arg₁     := .float
+  arg₂     := .float
   res      := .float
   f        := FloatBits.mul
+  dom      := fun _ _ => True
+  pre      := none
   defAxiom := binFloatDefAxiom floatMulSym .fpMul
 
 def floatMul : Intrinsic := floatMulB.toIntrinsic
@@ -342,21 +381,27 @@ def floatMul : Intrinsic := floatMulB.toIntrinsic
 @[simp] theorem floatMul_arity : floatMul.arity = .two := rfl
 
 def floatMulLawful : floatMulB.Lawful where
-  argL       := Embedding.lawfulFloat
-  resL       := Embedding.lawfulFloat
-  specBaseWf := by apply PredTrans.checkWf_ok; rfl
-  defWf      := by apply Formula.checkWf_ok; rfl
-  typeWf     := by apply Formula.checkWf_ok; rfl
-  defEval    := by intrinsic_def_eval [binTerm, floatMulB, floatMulSym, binFloatDefAxiom]; intros; rfl
+  argL₁        := Embedding.lawfulFloat
+  argL₂        := Embedding.lawfulFloat
+  resL         := Embedding.lawfulFloat
+  domSound     := fun _ _ _ _ => True.intro
+  semWellTyped := fun _ _ _ _ _ => sep_emp.1
+  specBaseWf   := by apply PredTrans.checkWf_ok; rfl
+  defWf        := by apply Formula.checkWf_ok; rfl
+  typeWf       := by intro φ h; injection h with h; subst h; apply Formula.checkWf_ok; rfl
+  defEval      := by intrinsic_def_eval [binTerm, floatMulB, floatMulSym, binFloatDefAxiom]; intros; rfl
 
 instance : IntrinsicSound [floatMul] floatMul := floatMulLawful.sound
 
 def floatDivB : Pure.Binary where
   name     := "float_div"
   path     := some ("Float", ["div"])
-  arg      := .float
+  arg₁     := .float
+  arg₂     := .float
   res      := .float
   f        := FloatBits.div
+  dom      := fun _ _ => True
+  pre      := none
   defAxiom := binFloatDefAxiom floatDivSym .fpDiv
 
 def floatDiv : Intrinsic := floatDivB.toIntrinsic
@@ -365,12 +410,15 @@ def floatDiv : Intrinsic := floatDivB.toIntrinsic
 @[simp] theorem floatDiv_arity : floatDiv.arity = .two := rfl
 
 def floatDivLawful : floatDivB.Lawful where
-  argL       := Embedding.lawfulFloat
-  resL       := Embedding.lawfulFloat
-  specBaseWf := by apply PredTrans.checkWf_ok; rfl
-  defWf      := by apply Formula.checkWf_ok; rfl
-  typeWf     := by apply Formula.checkWf_ok; rfl
-  defEval    := by intrinsic_def_eval [binTerm, floatDivB, floatDivSym, binFloatDefAxiom]; intros; rfl
+  argL₁        := Embedding.lawfulFloat
+  argL₂        := Embedding.lawfulFloat
+  resL         := Embedding.lawfulFloat
+  domSound     := fun _ _ _ _ => True.intro
+  semWellTyped := fun _ _ _ _ _ => sep_emp.1
+  specBaseWf   := by apply PredTrans.checkWf_ok; rfl
+  defWf        := by apply Formula.checkWf_ok; rfl
+  typeWf       := by intro φ h; injection h with h; subst h; apply Formula.checkWf_ok; rfl
+  defEval      := by intrinsic_def_eval [binTerm, floatDivB, floatDivSym, binFloatDefAxiom]; intros; rfl
 
 instance : IntrinsicSound [floatDiv] floatDiv := floatDivLawful.sound
 
@@ -390,9 +438,12 @@ def floatMinDefAxiom : Formula :=
 def floatMinB : Pure.Binary where
   name     := "float_min"
   path     := some ("Float", ["min"])
-  arg      := .float
+  arg₁     := .float
+  arg₂     := .float
   res      := .float
   f        := FloatBits.min
+  dom      := fun _ _ => True
+  pre      := none
   defAxiom := floatMinDefAxiom
 
 def floatMin : Intrinsic := floatMinB.toIntrinsic
@@ -401,12 +452,15 @@ def floatMin : Intrinsic := floatMinB.toIntrinsic
 @[simp] theorem floatMin_arity : floatMin.arity = .two := rfl
 
 def floatMinLawful : floatMinB.Lawful where
-  argL       := Embedding.lawfulFloat
-  resL       := Embedding.lawfulFloat
-  specBaseWf := by apply PredTrans.checkWf_ok; rfl
-  defWf      := by apply Formula.checkWf_ok; rfl
-  typeWf     := by apply Formula.checkWf_ok; rfl
-  defEval    := by intrinsic_def_eval [binTerm, floatMinB, floatMinDefAxiom, FloatBits.min]; intros; rfl
+  argL₁        := Embedding.lawfulFloat
+  argL₂        := Embedding.lawfulFloat
+  resL         := Embedding.lawfulFloat
+  domSound     := fun _ _ _ _ => True.intro
+  semWellTyped := fun _ _ _ _ _ => sep_emp.1
+  specBaseWf   := by apply PredTrans.checkWf_ok; rfl
+  defWf        := by apply Formula.checkWf_ok; rfl
+  typeWf       := by intro φ h; injection h with h; subst h; apply Formula.checkWf_ok; rfl
+  defEval      := by intrinsic_def_eval [binTerm, floatMinB, floatMinDefAxiom, FloatBits.min]; intros; rfl
 
 instance : IntrinsicSound [floatMin] floatMin := floatMinLawful.sound
 
@@ -426,9 +480,12 @@ def floatMaxDefAxiom : Formula :=
 def floatMaxB : Pure.Binary where
   name     := "float_max"
   path     := some ("Float", ["max"])
-  arg      := .float
+  arg₁     := .float
+  arg₂     := .float
   res      := .float
   f        := FloatBits.max
+  dom      := fun _ _ => True
+  pre      := none
   defAxiom := floatMaxDefAxiom
 
 def floatMax : Intrinsic := floatMaxB.toIntrinsic
@@ -437,12 +494,15 @@ def floatMax : Intrinsic := floatMaxB.toIntrinsic
 @[simp] theorem floatMax_arity : floatMax.arity = .two := rfl
 
 def floatMaxLawful : floatMaxB.Lawful where
-  argL       := Embedding.lawfulFloat
-  resL       := Embedding.lawfulFloat
-  specBaseWf := by apply PredTrans.checkWf_ok; rfl
-  defWf      := by apply Formula.checkWf_ok; rfl
-  typeWf     := by apply Formula.checkWf_ok; rfl
-  defEval    := by intrinsic_def_eval [binTerm, floatMaxB, floatMaxDefAxiom, FloatBits.max]; intros; rfl
+  argL₁        := Embedding.lawfulFloat
+  argL₂        := Embedding.lawfulFloat
+  resL         := Embedding.lawfulFloat
+  domSound     := fun _ _ _ _ => True.intro
+  semWellTyped := fun _ _ _ _ _ => sep_emp.1
+  specBaseWf   := by apply PredTrans.checkWf_ok; rfl
+  defWf        := by apply Formula.checkWf_ok; rfl
+  typeWf       := by intro φ h; injection h with h; subst h; apply Formula.checkWf_ok; rfl
+  defEval      := by intrinsic_def_eval [binTerm, floatMaxB, floatMaxDefAxiom, FloatBits.max]; intros; rfl
 
 instance : IntrinsicSound [floatMax] floatMax := floatMaxLawful.sound
 
@@ -455,9 +515,12 @@ private def binFloatBoolDefAxiom (sym : FOL.Symbol .two) (op : BinOp .float .flo
 def floatEqualB : Pure.Binary where
   name     := "float_equal"
   path     := some ("Float", ["equal"])
-  arg      := .float
+  arg₁     := .float
+  arg₂     := .float
   res      := .bool
   f        := FloatBits.eq
+  dom      := fun _ _ => True
+  pre      := none
   defAxiom := binFloatBoolDefAxiom floatEqualSym .fpEq
 
 def floatEqual : Intrinsic := floatEqualB.toIntrinsic
@@ -466,21 +529,27 @@ def floatEqual : Intrinsic := floatEqualB.toIntrinsic
 @[simp] theorem floatEqual_arity : floatEqual.arity = .two := rfl
 
 def floatEqualLawful : floatEqualB.Lawful where
-  argL       := Embedding.lawfulFloat
-  resL       := Embedding.lawfulBool
-  specBaseWf := by apply PredTrans.checkWf_ok; rfl
-  defWf      := by apply Formula.checkWf_ok; rfl
-  typeWf     := by apply Formula.checkWf_ok; rfl
-  defEval    := by intrinsic_def_eval [binTerm, floatEqualB, floatEqualSym, binFloatBoolDefAxiom]; intros; rfl
+  argL₁        := Embedding.lawfulFloat
+  argL₂        := Embedding.lawfulFloat
+  resL         := Embedding.lawfulBool
+  domSound     := fun _ _ _ _ => True.intro
+  semWellTyped := fun _ _ _ _ _ => sep_emp.1
+  specBaseWf   := by apply PredTrans.checkWf_ok; rfl
+  defWf        := by apply Formula.checkWf_ok; rfl
+  typeWf       := by intro φ h; injection h with h; subst h; apply Formula.checkWf_ok; rfl
+  defEval      := by intrinsic_def_eval [binTerm, floatEqualB, floatEqualSym, binFloatBoolDefAxiom]; intros; rfl
 
 instance : IntrinsicSound [floatEqual] floatEqual := floatEqualLawful.sound
 
 def floatLtB : Pure.Binary where
   name     := "float_lt"
   path     := some ("Float", ["lt"])
-  arg      := .float
+  arg₁     := .float
+  arg₂     := .float
   res      := .bool
   f        := FloatBits.lt
+  dom      := fun _ _ => True
+  pre      := none
   defAxiom := binFloatBoolDefAxiom floatLtSym .fpLt
 
 def floatLt : Intrinsic := floatLtB.toIntrinsic
@@ -489,21 +558,27 @@ def floatLt : Intrinsic := floatLtB.toIntrinsic
 @[simp] theorem floatLt_arity : floatLt.arity = .two := rfl
 
 def floatLtLawful : floatLtB.Lawful where
-  argL       := Embedding.lawfulFloat
-  resL       := Embedding.lawfulBool
-  specBaseWf := by apply PredTrans.checkWf_ok; rfl
-  defWf      := by apply Formula.checkWf_ok; rfl
-  typeWf     := by apply Formula.checkWf_ok; rfl
-  defEval    := by intrinsic_def_eval [binTerm, floatLtB, floatLtSym, binFloatBoolDefAxiom]; intros; rfl
+  argL₁        := Embedding.lawfulFloat
+  argL₂        := Embedding.lawfulFloat
+  resL         := Embedding.lawfulBool
+  domSound     := fun _ _ _ _ => True.intro
+  semWellTyped := fun _ _ _ _ _ => sep_emp.1
+  specBaseWf   := by apply PredTrans.checkWf_ok; rfl
+  defWf        := by apply Formula.checkWf_ok; rfl
+  typeWf       := by intro φ h; injection h with h; subst h; apply Formula.checkWf_ok; rfl
+  defEval      := by intrinsic_def_eval [binTerm, floatLtB, floatLtSym, binFloatBoolDefAxiom]; intros; rfl
 
 instance : IntrinsicSound [floatLt] floatLt := floatLtLawful.sound
 
 def floatLeB : Pure.Binary where
   name     := "float_le"
   path     := some ("Float", ["le"])
-  arg      := .float
+  arg₁     := .float
+  arg₂     := .float
   res      := .bool
   f        := FloatBits.le
+  dom      := fun _ _ => True
+  pre      := none
   defAxiom := binFloatBoolDefAxiom floatLeSym .fpLe
 
 def floatLe : Intrinsic := floatLeB.toIntrinsic
@@ -512,12 +587,15 @@ def floatLe : Intrinsic := floatLeB.toIntrinsic
 @[simp] theorem floatLe_arity : floatLe.arity = .two := rfl
 
 def floatLeLawful : floatLeB.Lawful where
-  argL       := Embedding.lawfulFloat
-  resL       := Embedding.lawfulBool
-  specBaseWf := by apply PredTrans.checkWf_ok; rfl
-  defWf      := by apply Formula.checkWf_ok; rfl
-  typeWf     := by apply Formula.checkWf_ok; rfl
-  defEval    := by intrinsic_def_eval [binTerm, floatLeB, floatLeSym, binFloatBoolDefAxiom]; intros; rfl
+  argL₁        := Embedding.lawfulFloat
+  argL₂        := Embedding.lawfulFloat
+  resL         := Embedding.lawfulBool
+  domSound     := fun _ _ _ _ => True.intro
+  semWellTyped := fun _ _ _ _ _ => sep_emp.1
+  specBaseWf   := by apply PredTrans.checkWf_ok; rfl
+  defWf        := by apply Formula.checkWf_ok; rfl
+  typeWf       := by intro φ h; injection h with h; subst h; apply Formula.checkWf_ok; rfl
+  defEval      := by intrinsic_def_eval [binTerm, floatLeB, floatLeSym, binFloatBoolDefAxiom]; intros; rfl
 
 instance : IntrinsicSound [floatLe] floatLe := floatLeLawful.sound
 
@@ -539,12 +617,13 @@ def floatNan : Intrinsic := floatNanB.toIntrinsic
 @[simp] theorem floatNan_arity : floatNan.arity = .zero := rfl
 
 def floatNanLawful : floatNanB.Lawful where
-  resL       := Embedding.lawfulFloat
-  nameFresh  := by decide
-  specBaseWf := by apply PredTrans.checkWf_ok; rfl
-  defWf      := by apply Formula.checkWf_ok; rfl
-  typeWf     := by apply Formula.checkWf_ok; rfl
-  defEval    := by intrinsic_def_eval [constTerm, floatNanB, floatNanSym, zeroFloatDefAxiom]
+  resL         := Embedding.lawfulFloat
+  nameFresh    := by decide
+  semWellTyped := fun _ _ => .rfl
+  specBaseWf   := by apply PredTrans.checkWf_ok; rfl
+  defWf        := by apply Formula.checkWf_ok; rfl
+  typeWf       := by intro φ h; injection h with h; subst h; apply Formula.checkWf_ok; rfl
+  defEval      := by intrinsic_def_eval [constTerm, floatNanB, floatNanSym, zeroFloatDefAxiom]
 
 instance : IntrinsicSound [floatNan] floatNan := floatNanLawful.sound
 
@@ -561,12 +640,13 @@ def floatInfinity : Intrinsic := floatInfinityB.toIntrinsic
 @[simp] theorem floatInfinity_arity : floatInfinity.arity = .zero := rfl
 
 def floatInfinityLawful : floatInfinityB.Lawful where
-  resL       := Embedding.lawfulFloat
-  nameFresh  := by decide
-  specBaseWf := by apply PredTrans.checkWf_ok; rfl
-  defWf      := by apply Formula.checkWf_ok; rfl
-  typeWf     := by apply Formula.checkWf_ok; rfl
-  defEval    := by intrinsic_def_eval [constTerm, floatInfinityB, floatInfinitySym, zeroFloatDefAxiom]
+  resL         := Embedding.lawfulFloat
+  nameFresh    := by decide
+  semWellTyped := fun _ _ => .rfl
+  specBaseWf   := by apply PredTrans.checkWf_ok; rfl
+  defWf        := by apply Formula.checkWf_ok; rfl
+  typeWf       := by intro φ h; injection h with h; subst h; apply Formula.checkWf_ok; rfl
+  defEval      := by intrinsic_def_eval [constTerm, floatInfinityB, floatInfinitySym, zeroFloatDefAxiom]
 
 instance : IntrinsicSound [floatInfinity] floatInfinity := floatInfinityLawful.sound
 
@@ -584,12 +664,13 @@ def floatNegInfinity : Intrinsic := floatNegInfinityB.toIntrinsic
 @[simp] theorem floatNegInfinity_arity : floatNegInfinity.arity = .zero := rfl
 
 def floatNegInfinityLawful : floatNegInfinityB.Lawful where
-  resL       := Embedding.lawfulFloat
-  nameFresh  := by decide
-  specBaseWf := by apply PredTrans.checkWf_ok; rfl
-  defWf      := by apply Formula.checkWf_ok; rfl
-  typeWf     := by apply Formula.checkWf_ok; rfl
-  defEval    := by intrinsic_def_eval [constTerm, floatNegInfinityB, floatNegInfinitySym, zeroFloatDefAxiom]
+  resL         := Embedding.lawfulFloat
+  nameFresh    := by decide
+  semWellTyped := fun _ _ => .rfl
+  specBaseWf   := by apply PredTrans.checkWf_ok; rfl
+  defWf        := by apply Formula.checkWf_ok; rfl
+  typeWf       := by intro φ h; injection h with h; subst h; apply Formula.checkWf_ok; rfl
+  defEval      := by intrinsic_def_eval [constTerm, floatNegInfinityB, floatNegInfinitySym, zeroFloatDefAxiom]
 
 instance : IntrinsicSound [floatNegInfinity] floatNegInfinity := floatNegInfinityLawful.sound
 
